@@ -931,6 +931,10 @@ import Xv6.FilewriteLoop
 import Xv6.FilewriteArms
 import Xv6.ProofFilewrite
 import Xv6.LinkFilewrite
+import Xv6.SpecSysWrite
+import Xv6.SysWriteParts
+import Xv6.ProofSysWrite
+import Xv6.LinkSysWrite
 import Xv6.KexecB
 import Xv6.KexecACode
 import Xv6.SpecSafestrcpySrc
